theories/rules/rules_Get.v
@@ -169,7 +169,8 @@ Section cap_lang_rules.
     iApply wp_wp2.
     iApply wp_opt2_bind.
     iApply wp_opt2_eqn.
-    iMod (state_interp_regs_transient_intro with "[$Hregs $Hσ]") as "Hσ".
+    iMod (state_interp_transient_intro (lm:= ∅) (df:= ∅) with "[$Hregs $Hσ]") as "Hσ";
+      [ rewrite prod_merge_empty_r ; iSplit ; [set_solver|done]|].
     iApply (wp2_reg_lookup (lrt := regs)); first by set_solver.
 
     iModIntro.
@@ -180,18 +181,18 @@ Section cap_lang_rules.
     iApply wp2_diag_univ.
     iSplit.
     { iIntros "%Hldn %Hdn".
-      iDestruct (state_interp_regs_transient_elim_abort with "Hσ") as "(Hσ & Hregs)".
+      iDestruct (state_interp_transient_elim_abort with "Hσ") as "(Hσ & Hregs & _)".
       iFrame.
       iApply ("Hφ" with "[$Hpc_a $Hregs]").
       iPureIntro. constructor.
       now eapply (Get_fail_src_denote _ _ _ _ _ Hlrs). }
-    
+
     iIntros (z Hdz _).
 
     iDestruct (update_state_interp_transient_from_regs_mod (dst := dst) (lw2 := LInt z) with "Hσ") as "Hσ".
     { now set_solver. }
-    { now intros. } 
-    
+    { now intros. }
+
     rewrite updatePC_incrementPC.
     iApply (wp_opt2_bind (φ1 := incrementLPC (<[ dst := LInt z]> regs)) (k1 := (fun x => Some x))).
     iApply wp_opt2_eqn_both.
@@ -199,7 +200,7 @@ Section cap_lang_rules.
     { rewrite dom_insert. apply elem_of_union_r. now rewrite elem_of_dom HPC. }
     iSplit.
     - iIntros (φt' lrt') "Hσ %Hlin %Hin".
-      iDestruct (state_interp_regs_transient_elim_abort with "Hσ") as "(Hσ & Hregs)".
+      iDestruct (state_interp_transient_elim_abort with "Hσ") as "(Hσ & Hregs & _)".
       iFrame.
       iApply ("Hφ" with "[$Hpc_a $Hregs]").
       iPureIntro.
@@ -208,7 +209,7 @@ Section cap_lang_rules.
     - iIntros (regs' φt') "Hσ %Hlis %His".
       iApply wp2_val.
       cbn.
-      iMod (state_interp_regs_transient_elim_commit with "Hσ") as "($ & Hregs)".
+      iMod (state_interp_transient_elim_commit with "Hσ") as "($ & Hregs & _)".
       iApply ("Hφ" with "[$Hpc_a $Hregs]").
       iPureIntro.
       eapply Get_spec_success; try eassumption.
